minor progress on mapping w/ layouts

mapper/SimpleMappingWithLayout.v
@@ -1,10 +1,11 @@
 Require Import SimpleMapping.
 Require Import MappingExamples.
+Require Import Utilities.
 
 Local Close Scope C_scope.
 Local Close Scope R_scope.
 
-(** Simple Mapping Extended with Layouts - WORK IN PROGRESS **)
+(** Simple Mapping Extended with Layouts **)
 
 (* This extends the simple mapping approach with a mapping between
    logical and physical qubits. In SimpleMapping, we moved logical 
@@ -45,21 +46,11 @@ Definition swap_in_map {dim} (m : qmap dim) phys1 phys2 : qmap dim :=
       (m1', m2')
   end.
 
-(* Copied from Coq.Logic.FinFun *)
-Definition bFun n (f : nat -> nat) := forall x, x < n -> f x < n.
-Definition bInjective n (f : nat -> nat) :=
- forall x y, x < n -> y < n -> f x = f y -> x = y.
-
-Definition bInverse n (f g : nat -> nat) := 
-  (forall x, x < n -> g (f x) = x) /\ (forall y, y < n -> f (g y) = y).
-
-(* Is there a more succinct way to write this? *)
+(* First two conditions necessary? *)
 Definition layout_well_formed {dim} (m : qmap dim) := 
-  bFun dim (log2phys m) /\
-  bFun dim (phys2log m) /\
-  bInjective dim (log2phys m) /\
-  bInjective dim (phys2log m) /\
-  bInverse dim (log2phys m) (phys2log m).
+  (forall x, x < dim <-> log2phys m x < dim) /\
+  (forall x, x < dim <-> phys2log m x < dim) /\
+  (forall x y, log2phys m x = y <-> phys2log m y = x).
 
 (* Mapping function definition. *)
 
@@ -69,9 +60,12 @@ Fixpoint path_to_swaps dim p m : (base_ucom dim * qmap dim) :=
   | n1 :: ((n2 :: _) as t) => 
       let (c, m') := path_to_swaps dim t (swap_in_map m n1 n2) in
       (SWAP n1 n2 ; c, m')
-  | _ => (SKIP, m) (* bad input case *)
+  | _ => (SKIP, m) (* bad input case - invaid path *)
   end.
 
+(* Note: the input program references *logical* qubits, and the returned program
+   references *physical* qubits. get_path and is_in_graph_b also reference physical
+   qubits. *)
 Fixpoint simple_map_w_layout {dim} (c : base_ucom dim) (m : qmap dim) (get_path : nat -> nat -> list nat) (is_in_graph_b : nat -> nat -> bool) : (base_ucom dim * qmap dim) :=
   match c with
   | c1; c2 => let (c1', m') := simple_map_w_layout c1 m get_path is_in_graph_b in
@@ -90,7 +84,9 @@ Fixpoint simple_map_w_layout {dim} (c : base_ucom dim) (m : qmap dim) (get_path 
    to the input program if you 'undo' all the SWAPs. To state this, we need a 
    way to produce a series of SWAPs that converts between layouts. *)
 
-(* If the m1 has logical qubit A at physical qubit 0 and m2 has A at 3, 
+(* The goal is to get from layout m1 to layout m2.
+   
+   If the m1 has logical qubit A at physical qubit 0 and m2 has A at 3, 
    then convert_between_layouts should produce a program that swaps the
    values at locations 0 and 3. Note that we don't worry about satisfying
    connectivity constraints because the generated program is used in our
@@ -108,7 +104,7 @@ Fixpoint convert_between_layouts' {dim} n (m1 m2 : qmap dim) : base_ucom dim :=
 Definition convert_between_layouts {dim} (m1 m2 : qmap dim) : base_ucom dim :=
   convert_between_layouts' dim m1 m2.
 
-(* Example *)
+(* Examples *)
 Definition trivial_layout : qmap 5 := (fun x => x, fun x => x).
 Definition test_layout1 : qmap 5 := 
   let l2p q := if q =? 0 then 4
@@ -126,27 +122,6 @@ Compute (convert_between_layouts trivial_layout test_layout1).
 Compute (convert_between_layouts test_layout1 trivial_layout).
 Compute (convert_between_layouts test_layout1 test_layout1).
 
-(* The statements of correctness will probably look like the following: *)
-Lemma simple_map_w_layout_sound : forall dim (c : base_ucom dim) (m : qmap dim) get_path is_in_graph is_in_graph_b c' m',
-  valid_graph dim is_in_graph ->
-  get_path_valid dim get_path is_in_graph ->
-  (forall n1 n2, reflect (is_in_graph n1 n2) (is_in_graph_b n1 n2)) ->
-  uc_well_typed c ->
-  layout_well_formed m ->
-  simple_map_w_layout c m get_path is_in_graph_b = (c', m') -> 
-  (c' ; convert_between_layouts m' m) ≡ (map_qubits (log2phys m) c).
-Proof. Admitted.
-
-Lemma simple_map_w_layout_respect_constraints : forall dim (c : base_ucom dim) (m : qmap dim) get_path is_in_graph is_in_graph_b c' m',
-  valid_graph dim is_in_graph ->
-  get_path_valid dim get_path is_in_graph ->
-  (forall n1 n2, reflect (is_in_graph n1 n2) (is_in_graph_b n1 n2)) ->
-  uc_well_typed c ->
-  layout_well_formed m ->
-  simple_map_w_layout c m get_path is_in_graph_b = (c', m') -> 
-  respects_constraints is_in_graph c'.
-Proof. Admitted.
-
 Definition map_to_tenerife_w_layout (c : base_ucom 5) (m : qmap 5) :=
   simple_map_w_layout c m Tenerife.tenerife_get_path Tenerife.tenerife_is_in_graph_b.
 
@@ -157,8 +132,8 @@ Compute (map_to_tenerife_w_layout Tenerife.test_tenerife2 test_layout1).
 Compute (map_to_tenerife_w_layout Tenerife.test_tenerife3 trivial_layout).
 Compute (map_to_tenerife_w_layout Tenerife.test_tenerife3 test_layout1).
 
-(* Represent a layout as a list where element x at index i indicates
-   that logical qubit x is located at physical qubit i.  *)
+(* Represent a layout as a list where element x at index i indicates that
+   logical qubit x is located at physical qubit i. (Makes printing nicer.)  *)
 Fixpoint layout_to_list' {dim} n (m : qmap dim) :=
   match n with 
   | O => []
@@ -169,14 +144,489 @@ Definition layout_to_list {dim} (m : qmap dim) := layout_to_list' dim m.
 Compute (layout_to_list trivial_layout).
 Compute (layout_to_list test_layout1).
 
-Fixpoint layout_from_list' n l :=
-  match l with 
-  | [] => (fun x => x, fun x => x)
-  | h :: t => let (l2p, p2l) := layout_from_list' (n+1) t in
-            let l2p' x := if x =? h then n else l2p x in
-            let p2l' x := if x =? n then h else p2l x in
-            (l2p', p2l')   
-  end.
-Definition layout_from_list dim l : (qmap dim) := layout_from_list' 0 l.
+(* Proofs *)
 
-Compute (layout_to_list (layout_from_list 5 (3 :: 4 :: 1 :: 2 :: 0 :: []))).
+Lemma swap_in_map_well_formed : forall {dim} (m : qmap dim) n1 n2,
+  n1 < dim -> n2 < dim -> layout_well_formed m -> 
+  layout_well_formed (swap_in_map m n1 n2).
+Proof.
+  unfold layout_well_formed, swap_in_map, log2phys, phys2log.
+  intros dim m n1 n2 Hn1 Hn2.
+  destruct m as [m1 m2].
+  intros [H1 [H2 H3]].
+  repeat split; intros H.
+  - bdestruct (x =? m2 n1). assumption.
+    bdestruct (x =? m2 n2). assumption.
+    rewrite <- H1. assumption.
+  - bdestruct (x =? m2 n1). subst. rewrite <- H2. assumption.
+    bdestruct (x =? m2 n2). subst. rewrite <- H2. assumption.
+    rewrite <- H1 in H. assumption.
+  - bdestruct (x =? n1). rewrite <- H2. assumption.
+    bdestruct (x =? n2). rewrite <- H2. assumption.
+    rewrite <- H2. assumption.
+  - bdestruct (x =? n1). subst. assumption.
+    bdestruct (x =? n2). subst. assumption.
+    rewrite <- H2 in H. assumption.
+  - bdestruct (x =? m2 n1); subst.
+    bdestruct (y =? n1); subst. 
+    reflexivity.
+    bdestructΩ (y =? y).  
+    bdestruct (x =? m2 n2); subst.
+    bdestructΩ (n1 =? n1).
+    apply not_eq_sym in H0.    
+    rewrite <- H3 in H0; try assumption.
+    apply not_eq_sym in H.
+    rewrite <- H3 in H; try assumption.
+    bdestructΩ (m1 x =? n1); bdestructΩ (m1 x =? n2).
+    apply H3; auto.
+  - bdestruct (y =? n1); subst.
+    bdestruct (m2 n2 =? m2 n1); subst.
+    symmetry in H; apply H3 in H; try assumption.
+    rewrite <- H.
+    symmetry; apply H3; auto.
+    bdestructΩ (m2 n2 =? m2 n2).
+    bdestruct (y =? n2); subst.
+    bdestructΩ (m2 n1 =? m2 n1).
+    apply not_eq_sym in H0.
+    bdestruct (m2 y =? m2 n1); subst.
+    symmetry in H1; apply H3 in H4; auto.
+    contradict H0.
+    rewrite <- H4.
+    symmetry.
+    apply H3; auto.
+    bdestruct (m2 y =? m2 n2); subst.
+    symmetry; apply H3 in H5; auto.
+    contradict H.
+    rewrite <- H5.
+    apply H3; auto.
+    apply H3; auto.    
+Qed.
+
+Lemma swap_in_map_twice : forall {dim} (m : qmap dim) n1 n2,
+  layout_well_formed m ->
+  swap_in_map (swap_in_map m n1 n2) n1 n2 = m.
+Proof.
+  intros dim m n1 n2 [_ [_ WF]].
+  unfold swap_in_map.
+  destruct m.
+  simpl in WF.
+  bdestructΩ (n1 =? n1).
+  bdestructΩ (n2 =? n2).
+  apply f_equal2.
+  - apply functional_extensionality.
+    intros x.
+    bdestruct (x =? n0 n2).
+    symmetry. apply WF. auto.
+    bdestruct (n2 =? n1); subst.
+    bdestructΩ (x =? n0 n1).
+    bdestruct (x =? n0 n1); auto.
+    symmetry. apply WF. auto.
+  - apply functional_extensionality.
+    intros x.
+    bdestruct (x =? n1); subst.
+    bdestruct (n2 =? n1); subst; auto.
+    bdestruct (x =? n2); subst; auto.
+Qed.
+
+Lemma convert_between_layouts'_same : forall {dim} n (m : qmap dim),
+  layout_well_formed m -> convert_between_layouts' n m m ≡ SKIP.
+Proof.
+  intros dim n m [_ [_ WF]].
+  induction n.
+  reflexivity.
+  simpl. 
+  bdestruct (n =? log2phys m (phys2log m n)).
+  apply IHn.
+  contradict H. 
+  symmetry. apply WF. reflexivity.
+Qed.
+
+Lemma convert_between_layouts_same : forall {dim} (m : qmap dim),
+  layout_well_formed m -> convert_between_layouts m m ≡ SKIP.
+Proof. intros. apply convert_between_layouts'_same. assumption. Qed.
+
+Lemma convert_between_layouts'_SWAP : forall {dim} n (m1 m2 : qmap dim) n1 n2,
+  layout_well_formed m1 ->
+  layout_well_formed m2 ->
+  n1 < dim -> n2 < dim -> n1 <> n2 -> (* SWAP n1 n2 is well typed *)
+  (* some restriction involving n... *)
+  SWAP n1 n2 ; convert_between_layouts' n (swap_in_map m1 n1 n2) m2 ≡ convert_between_layouts' n m1 m2.
+Proof. Admitted.
+
+Lemma convert_between_layouts_SWAP : forall {dim} (m1 m2 : qmap dim) n1 n2,
+  layout_well_formed m1 ->
+  layout_well_formed m2 ->
+  n1 < dim -> n2 < dim -> n1 <> n2 ->
+  SWAP n1 n2 ; convert_between_layouts (swap_in_map m1 n1 n2) m2 ≡ convert_between_layouts m1 m2.
+Proof. intros. apply convert_between_layouts'_SWAP; assumption. Qed.
+
+Lemma convert_between_layouts_map_commutes : forall {dim} (m1 m2 : qmap dim) (c : base_ucom dim),
+  layout_well_formed m1 ->
+  layout_well_formed m2 ->
+  uc_well_typed c ->
+  convert_between_layouts m1 m2 ; map_qubits (log2phys m2) c ≡ map_qubits (log2phys m1) c ; convert_between_layouts m1 m2.
+Proof.
+Admitted.
+
+Lemma convert_between_layouts_transitive : forall {dim} (m1 m2 m3 : qmap dim),
+  convert_between_layouts m1 m2 ; convert_between_layouts m2 m3 ≡ convert_between_layouts m1 m3.
+Proof.
+Admitted.
+
+Lemma path_to_swaps_well_formed : forall {dim} n1 n2 is_in_graph p m c m',
+  valid_graph dim is_in_graph ->
+  valid_path n1 n2 is_in_graph p ->
+  layout_well_formed m ->
+  path_to_swaps dim p m = (c, m') ->
+  layout_well_formed m'.
+Proof.
+  intros.
+  generalize dependent c.
+  generalize dependent m.
+  generalize dependent n1.
+  induction p; intros n1 Hpath m WFm c res; simpl in res.
+  inversion res; subst. assumption.
+  destruct p. inversion res; subst. assumption.
+  destruct p. inversion res; subst. assumption.
+  destruct (path_to_swaps dim (n :: n0 :: p) (swap_in_map m a n)) eqn:res'.
+  inversion res; subst.
+  destruct Hpath as [H1 [H2 [H3 H4]]].
+  inversion H1; subst.
+  eapply IHp; try apply res'.
+  repeat split.
+  inversion H2; subst. assumption.
+  inversion H3; subst. assumption. 
+  inversion H4; subst. assumption.
+  assert (a < dim).
+  { inversion H3; subst.
+    destruct H8.
+    apply H in H0 as [H0 _].
+    assumption. 
+    apply H in H0 as [_ [H0 _]]. 
+    assumption. }
+  assert (n < dim).
+  { inversion H3; subst.
+    destruct H9.
+    apply H in H5 as [_ [H5 _]].
+    assumption. 
+    apply H in H5 as [H5 _]. 
+    assumption. }
+  apply swap_in_map_well_formed; assumption.
+Qed.
+
+Lemma simple_map_w_layout_well_formed : forall {dim} (c : base_ucom dim) m get_path is_in_graph is_in_graph_b c' m',
+  valid_graph dim is_in_graph ->
+  get_path_valid dim get_path is_in_graph ->
+  (forall n1 n2, reflect (is_in_graph n1 n2) (is_in_graph_b n1 n2)) ->
+  uc_well_typed c ->
+  layout_well_formed m ->
+  simple_map_w_layout c m get_path is_in_graph_b = (c', m') ->
+  layout_well_formed m'.
+Proof.
+  intros dim c m get_path is_in_graph is_in_graph_b c' m' Hgraph Hpath Href WT WF res.
+  generalize dependent m'.
+  generalize dependent c'.
+  generalize dependent m.
+  induction c; intros m WF c' m' res; simpl in res.
+  - destruct (simple_map_w_layout c1 m get_path is_in_graph_b) eqn:res1.
+    destruct (simple_map_w_layout c2 q get_path is_in_graph_b) eqn:res2.
+    inversion res; subst.
+    inversion WT; subst.
+    eapply IHc2; try apply res2; auto.
+    eapply IHc1; try apply res1; auto.
+  - inversion res; subst. assumption.
+  - dependent destruction u.
+    destruct (path_to_swaps dim (get_path (log2phys m n) (log2phys m n0)) m) eqn:res'.
+    inversion res; subst.
+    eapply path_to_swaps_well_formed; try apply res'; auto.
+    apply Hgraph.
+    inversion WT; subst.
+    destruct WF as [WF1 [WF2 WF3]].
+    apply Hpath.
+    rewrite <- WF1; auto.
+    rewrite <- WF1; auto.
+    intros contra.
+    contradict H4.
+    apply WF3 in contra.
+    rewrite <- contra. 
+    apply WF3; auto.
+  - dependent destruction u.
+Qed.
+
+Lemma path_to_swaps_sound : forall {dim} n1 n2 is_in_graph p m c m',
+  valid_graph dim is_in_graph ->
+  valid_path n1 n2 is_in_graph p ->
+  layout_well_formed m ->
+  path_to_swaps dim p m = (c, m') ->
+  c ≡ convert_between_layouts m m'.
+Proof.
+  intros dim n1 n2 is_in_graph p m c m' Hgraph Hpath WF res.
+  generalize dependent c.
+  generalize dependent m.
+  generalize dependent n1.
+  induction p; intros n1 Hpath m WF c res; simpl in res.
+  destruct Hpath as [H _].
+  inversion H.
+  destruct p.
+  destruct Hpath as [_ [_ [H _]]].
+  inversion H.
+  destruct p.
+  inversion res; subst. symmetry. 
+  apply convert_between_layouts_same; assumption.
+  destruct (path_to_swaps dim (n :: n0 :: p) (swap_in_map m a n)) eqn:res'.
+  inversion res; subst.  
+  destruct Hpath as [H1 [H2 [H3 H4]]].
+  inversion H1; subst.
+  assert (a < dim).
+  { inversion H3; subst.
+    destruct H7.
+    apply Hgraph in H as [H _].
+    assumption. 
+    apply Hgraph in H as [_ [H _]]. 
+    assumption. }
+  assert (n < dim).
+  { inversion H3; subst.
+    destruct H8.
+    apply Hgraph in H0 as [_ [H0 _]].
+    assumption. 
+    apply Hgraph in H0 as [H0 _]. 
+    assumption. }
+  assert (a <> n).
+  { inversion H3; subst.
+    destruct H9.
+    apply Hgraph in H5 as [_ [_ H5]].
+    assumption. 
+    apply Hgraph in H5 as [_ [_ H5]]. 
+    lia. }
+  rewrite IHp with (c:=b); try apply res'.
+  apply convert_between_layouts_SWAP; auto.
+  eapply path_to_swaps_well_formed; try apply res'.
+  apply Hgraph.
+  repeat split.
+  inversion H2; subst. apply H8.
+  inversion H3; subst. assumption. 
+  inversion H4; subst. assumption.  
+  apply swap_in_map_well_formed; assumption.
+  repeat split.
+  inversion H2; subst. apply H8.
+  inversion H3; subst. assumption. 
+  inversion H4; subst. assumption.  
+  apply swap_in_map_well_formed; assumption.
+Qed.
+
+Lemma simple_map_w_layout_sound : forall dim (c : base_ucom dim) (m : qmap dim) get_path is_in_graph is_in_graph_b c' m',
+  valid_graph dim is_in_graph ->
+  get_path_valid dim get_path is_in_graph ->
+  (forall n1 n2, reflect (is_in_graph n1 n2) (is_in_graph_b n1 n2)) ->
+  uc_well_typed c ->
+  layout_well_formed m ->
+  simple_map_w_layout c m get_path is_in_graph_b = (c', m') -> 
+  (c' ; convert_between_layouts m' m) ≡ (map_qubits (log2phys m) c).
+Proof. 
+  intros dim c m get_path is_in_graph is_in_graph_b c' m' Hgraph Hpath Href WT WF res.
+  generalize dependent m'.
+  generalize dependent c'.
+  generalize dependent m.
+  induction c; intros m WF c' m' res.
+  - simpl in res. 
+    destruct (simple_map_w_layout c1 m get_path is_in_graph_b) eqn:res1.
+    destruct (simple_map_w_layout c2 q get_path is_in_graph_b) eqn:res2.
+    inversion res; subst.
+    simpl.
+    inversion WT; subst.
+    erewrite <- IHc1; try apply res1; auto.
+    repeat rewrite useq_assoc.
+    rewrite convert_between_layouts_map_commutes; try assumption.
+    erewrite <- IHc2; try apply res2; auto.
+    repeat rewrite useq_assoc.
+    rewrite convert_between_layouts_transitive.
+    reflexivity.
+    eapply simple_map_w_layout_well_formed; try apply res1; auto; assumption.
+    eapply simple_map_w_layout_well_formed; try apply res1; auto; assumption.
+  - inversion res; subst.
+    dependent destruction u. 
+    simpl.
+    apply uc_well_typed_implies_dim_nonzero in WT.
+    unfold convert_between_layouts.
+    rewrite convert_between_layouts'_same; try assumption.
+    unfold uc_equiv; simpl.
+    rewrite denote_SKIP; try assumption.
+    Msimpl_light; reflexivity.
+  - dependent destruction u. 
+    simpl in res.
+    destruct (path_to_swaps dim (get_path (log2phys m n) (log2phys m n0)) m) eqn:path.
+    inversion res; subst.
+    simpl.
+    repeat rewrite fix_cnots_sound.
+    Transparent CNOT.
+    replace (CNOT (log2phys m' n) (log2phys m' n0)) with (@map_qubits _ dim (log2phys m') (CNOT n n0)) by reflexivity.
+    rewrite useq_assoc.
+    rewrite <- convert_between_layouts_map_commutes; try assumption.
+    rewrite <- useq_assoc.
+    rewrite path_to_swaps_sound with (c:=b); try apply path; auto.
+    rewrite convert_between_layouts_transitive.
+    unfold convert_between_layouts.
+    rewrite convert_between_layouts'_same; try assumption.
+    unfold uc_equiv; simpl.
+    rewrite denote_SKIP.
+    Msimpl_light; reflexivity.
+    apply uc_well_typed_implies_dim_nonzero in WT. assumption.
+    apply Hgraph.
+    inversion WT; subst.
+    destruct WF as [WF1 [WF2 WF3]].
+    apply Hpath.
+    rewrite <- WF1; auto.
+    rewrite <- WF1; auto.
+    intros contra.
+    contradict H4.
+    apply WF3 in contra.
+    rewrite <- contra. 
+    apply WF3; auto.
+    eapply path_to_swaps_well_formed; try apply path; auto.
+    apply Hgraph.
+    inversion WT; subst.
+    destruct WF as [WF1 [WF2 WF3]].
+    apply Hpath.
+    rewrite <- WF1; auto.
+    rewrite <- WF1; auto.
+    intros contra.
+    contradict H4.
+    apply WF3 in contra.
+    rewrite <- contra. 
+    apply WF3; auto.
+  - dependent destruction u.
+Qed.
+
+Lemma path_to_swaps_respects_undirected : forall {dim} n1 n2 is_in_graph p m c m',
+  valid_graph dim is_in_graph ->
+  valid_path (log2phys m n1) (log2phys m n2) is_in_graph p ->
+  layout_well_formed m ->
+  path_to_swaps dim p m = (c, m') ->
+  respects_constraints_undirected is_in_graph (c ; CNOT (log2phys m' n1) (log2phys m' n2)).
+Proof.
+  intros dim n1 n2 is_in_graph p m c m' Hgraph Hpath WF res.
+  generalize dependent c.
+  generalize dependent m.
+  generalize dependent n1.
+  induction p; intros n1 m Hpath WF c res; simpl in res.
+  destruct Hpath as [H _].
+  inversion H.
+  destruct p.
+  destruct Hpath as [_ [_ [H _]]].
+  inversion H.
+  destruct p.
+  inversion res; subst. 
+  Transparent SKIP ID.
+  constructor; constructor.
+  destruct Hpath as [H1 [H2 [H3 H4]]].
+  inversion H1; subst.
+  inversion H2; subst.
+  inversion H5; subst.
+  inversion H3; subst.
+  assumption.
+  inversion H9. inversion H6.
+  destruct (path_to_swaps dim (n :: n0 :: p) (swap_in_map m a n)) eqn:res'.
+  inversion res; subst.
+  destruct Hpath as [H1 [H2 [H3 H4]]].
+  inversion H1; subst.
+  inversion H3; subst.
+  assert (log2phys m n1 < dim).
+  { destruct H7.
+    apply Hgraph in H as [H _].
+    assumption. 
+    apply Hgraph in H as [_ [H _]]. 
+    assumption. }
+  assert (n < dim).
+  { destruct H7.
+    apply Hgraph in H0 as [_ [H0 _]].
+    assumption. 
+    apply Hgraph in H0 as [H0 _]. 
+    assumption. }
+  assert (aux: forall (a b c : base_ucom dim), 
+    respects_constraints_undirected is_in_graph ((a;b);c) <-> respects_constraints_undirected is_in_graph (a;(b;c))).
+  { clear. intros a b c. split; intros H. 
+    inversion H; subst. inversion H3; subst.
+    repeat constructor; auto.
+    inversion H; subst. inversion H4; subst.
+    repeat constructor; auto. }
+  apply aux.
+  constructor.
+  Transparent SWAP.
+  repeat apply res_und_seq; constructor; auto.
+  apply or_comm; assumption.
+  eapply IHp; try apply res'.
+  replace (log2phys (swap_in_map m (log2phys m n1) n) n1) with n.
+  2: { unfold swap_in_map. 
+       destruct m; simpl.
+       destruct WF as [_ [_ WF]].
+       bdestruct (n1 =? n4 (n3 n1)).
+       reflexivity.
+       contradict H5.
+       symmetry. apply WF. reflexivity. }
+  replace (log2phys (swap_in_map m (log2phys m n1) n) n2) with (log2phys m n2).
+  2: { unfold swap_in_map. 
+       destruct m; simpl.
+       destruct WF as [_ [_ WF]]. 
+       inversion H4; subst.
+       bdestruct (n2 =? n4 (n3 n1)).
+       symmetry in H5.
+       apply WF in H5.
+       contradict H10. symmetry. assumption.
+       bdestruct (n2 =? n4 n).
+       inversion H12; subst.
+       contradict H13. symmetry. apply WF. reflexivity.
+       contradict H14. symmetry. apply WF. reflexivity.
+       reflexivity. }
+  repeat split.
+  inversion H2; subst. assumption.
+  inversion H3; subst. assumption. 
+  inversion H4; subst. assumption.  
+  apply swap_in_map_well_formed; assumption.
+Qed.
+  
+Lemma simple_map_w_layout_respects_constraints : forall dim (c : base_ucom dim) (m : qmap dim) get_path is_in_graph is_in_graph_b c' m',
+  valid_graph dim is_in_graph ->
+  get_path_valid dim get_path is_in_graph ->
+  (forall n1 n2, reflect (is_in_graph n1 n2) (is_in_graph_b n1 n2)) ->
+  uc_well_typed c ->
+  layout_well_formed m ->
+  simple_map_w_layout c m get_path is_in_graph_b = (c', m') -> 
+  respects_constraints is_in_graph c'.
+Proof. 
+  intros dim c m get_path is_in_graph is_in_graph_b c' m' Hgraph Hpath Href WT WF res.
+  generalize dependent m'.
+  generalize dependent c'.
+  generalize dependent m.
+  induction c; intros m WF c' m' res.
+  - inversion WT; subst.
+    simpl in res. 
+    destruct (simple_map_w_layout c1 m get_path is_in_graph_b) eqn:res1.
+    destruct (simple_map_w_layout c2 q get_path is_in_graph_b) eqn:res2.
+    inversion res; subst.
+    constructor.
+    eapply IHc1; try apply res1; auto.
+    eapply IHc2; try apply res2; auto.
+    eapply simple_map_w_layout_well_formed; try apply res1; auto; assumption.
+  - inversion res; subst. constructor.
+  - dependent destruction u.
+    Opaque fix_cnots. 
+    simpl in res.
+    destruct (path_to_swaps dim (get_path (log2phys m n) (log2phys m n0)) m) eqn:path.
+    inversion res; subst.
+    apply fix_cnots_respects_constraints; try assumption. 
+    eapply path_to_swaps_respects_undirected; try apply path; auto.
+    inversion WT; subst.
+    destruct WF as [WF1 [WF2 WF3]].
+    apply Hpath.
+    rewrite <- WF1; auto.
+    rewrite <- WF1; auto.
+    intros contra.
+    contradict H4.
+    apply WF3 in contra.
+    rewrite <- contra. 
+    apply WF3; auto.
+  - dependent destruction u.
+Qed.
+
+
+
